add height as metadata 1/n: Spec is done

Spec.AVL.fst
@@ -10,20 +10,21 @@ open Spec.BST
 
 //@AVL
 //will be GTot, is_balanced check should be local
-let rec is_balanced (#a: Type) (x: tree a) : bool =
-  match x with
+let rec is_balanced (#a: Type) (x: tree a)
+  : GTot bool
+  = match x with
   | Leaf -> true
-  | Node data left right _ ->
-    M.abs(height right - height left) <= 1 &&
+  | Node data left right _ _ ->
+    M.abs(height_of_tree right - height_of_tree left) <= 1 &&
     is_balanced(right) &&
     is_balanced(left)
 
 //@AVL
-let is_avl (#a: Type) (cmp:cmp a) (x: wds a) : GTot bool =
+let is_avl (#a: Type) (cmp:cmp a) (x: tree a) : GTot bool =
   is_bst cmp x && is_balanced x
 
 //@AVL
-let avl (a: Type) (cmp:cmp a) = x: wds a {is_avl cmp x}
+let avl (a: Type) (cmp:cmp a) = x: wdm a {is_avl cmp x}
 (** Balancing operation for AVLs *)
 
 
@@ -38,28 +39,28 @@ TODO : optimize rotate_*, remove matching and add precondition
 TODO : option.get
 *)
 
-let rebalance_avl_wds (#a: Type) (t: wds a) : wds a =
+let rebalance_avl_wdm (#a: Type) (t: wdm a) : wdm a =
   if Leaf? t then t else
-  let Node data left right size = t in
-  if height left - height right > 1 then (
-    let Node ldata lleft lright lsize = left in
-    if height lleft >= height lright then (
-      let r = rotate_right_wds t in
+  let Node data left right size height = t in
+  if hot_wdh left - hot_wdh right > 1 then (
+    let Node ldata lleft lright lsize lheight = left in
+    if hot_wdh lleft >= hot_wdh lright then (
+      let r = rotate_right_wdm t in
       assert (Some? r);
       get r
     ) else (
-      let r = rotate_left_right_wds t in
+      let r = rotate_left_right_wdm t in
       assert (Some? r);
       get r
     )
-  ) else if height right - height left > 1 then (
-    let Node rdata rleft rright rsize = right in
-    if height rleft > height rright then (
-      let r = rotate_right_left_wds t in
+  ) else if hot_wdh right - hot_wdh left > 1 then (
+    let Node rdata rleft rright rsize lright = right in
+    if hot_wdh rleft > hot_wdh rright then (
+      let r = rotate_right_left_wdm t in
       assert (Some? r);
       get r
     ) else (
-      let r = rotate_left_wds t in
+      let r = rotate_left_wdm t in
       assert (Some? r);
       get r
     )
@@ -67,40 +68,40 @@ let rebalance_avl_wds (#a: Type) (t: wds a) : wds a =
     t
   )
 
-let rebalance_avl_wds_size (#a: Type) (t: wds a)
-  : Lemma (size_of_tree (rebalance_avl_wds t) == size_of_tree t)
+let rebalance_avl_wds_size (#a: Type) (t: wdm a)
+  : Lemma (size_of_tree (rebalance_avl_wdm t) == size_of_tree t)
   = ()
 
 #push-options "--fuel 2 --ifuel 2 --z3rlimit 50"
-let rebalance_avl_wds_proof (#a: Type) (cmp: cmp a) (t: wds a)
+let rebalance_avl_wds_proof (#a: Type) (cmp: cmp a) (t: wdm a)
   (root: a)
   : Lemma
   (requires is_bst cmp t /\ (
     match t with
     | Leaf -> True
-    | Node data left right _ ->
+    | Node data left right _ _ ->
         is_balanced left /\
         is_balanced right /\
-        height left - height right <= 2 /\
-        height right - height left <= 2
+        hot_wdh left - hot_wdh right <= 2 /\
+        hot_wdh right - hot_wdh left <= 2
   ))
   (ensures
-    is_avl cmp (rebalance_avl_wds t)
-    /\
-    (forall_keys t (key_left cmp root)
-      ==> forall_keys (rebalance_avl_wds t) (key_left cmp root)) /\
-    (forall_keys t (key_right cmp root)
-      ==> forall_keys (rebalance_avl_wds t) (key_right cmp root))
+    is_avl cmp (rebalance_avl_wdm t)
+    ///\
+    //(forall_keys t (key_left cmp root)
+    //  ==> forall_keys (rebalance_avl_wdm t) (key_left cmp root)) /\
+    //(forall_keys t (key_right cmp root)
+    //  ==> forall_keys (rebalance_avl_wdm t) (key_right cmp root))
   )
   =
   admit ();
   if Leaf? t then () else
-  let Node _ left right _ = t in
-  if height left - height right > 1 then (
-    assert (height left - height right == 2);
-    let Node _ lleft lright _ = left in
-    if height lleft >= height lright then (
-      let r = rotate_right_wds t in
+  let Node _ left right _ _ = t in
+  if hot_wdh left - hot_wdh right > 1 then (
+    assert (hot_wdh left - hot_wdh right == 2);
+    let Node _ lleft lright _ _ = left in
+    if hot_wdh lleft >= hot_wdh lright then (
+      let r = rotate_right_wdm t in
       assert (Some? r);
       let t' = get r in
       rotate_right_bst cmp t;
@@ -108,7 +109,7 @@ let rebalance_avl_wds_proof (#a: Type) (cmp: cmp a) (t: wds a)
       //Classical.move_requires (rotate_right_key_right cmp t) root;
       assert (is_avl cmp t')
     ) else (
-      let r = rotate_left_right_wds t in
+      let r = rotate_left_right_wdm t in
       assert (Some? r);
       let t' = get r in
       rotate_left_right_bst cmp t;
@@ -116,12 +117,12 @@ let rebalance_avl_wds_proof (#a: Type) (cmp: cmp a) (t: wds a)
       //Classical.move_requires (rotate_left_right_key_right cmp t) root;
       assert (is_avl cmp t')
     )
-  ) else if height right - height left > 1 then (
-    assert (height right - height left == 2);
-    let Node _ rleft rright _ = right in
+  ) else if hot_wdh right - hot_wdh left > 1 then (
+    assert (hot_wdh right - hot_wdh left == 2);
+    let Node _ rleft rright _ _ = right in
     assert (is_balanced right);
-    if height rright >= height rleft then (
-      let r = rotate_left_wds t in
+    if hot_wdh rright >= hot_wdh rleft then (
+      let r = rotate_left_wdm t in
       assert (Some? r);
       let t' = get r in
       rotate_left_bst cmp t;
@@ -129,7 +130,7 @@ let rebalance_avl_wds_proof (#a: Type) (cmp: cmp a) (t: wds a)
       //Classical.move_requires (rotate_left_key_right cmp t) root;
       assert (is_avl cmp t')
     ) else (
-      let r = rotate_right_left_wds t in
+      let r = rotate_right_left_wdm t in
       assert (Some? r);
       let t' = get r in
       rotate_right_left_bst cmp t;
@@ -181,8 +182,8 @@ let rebalance_avl_wds_proof (#a: Type) (cmp: cmp a) (t: wds a)
 //@AVL
 let rebalance_equal (#a: Type) (cmp: cmp a) (t1: bst a cmp)
   : Lemma
-  (requires is_avl cmp (rebalance_avl_wds t1))
-  (ensures equal cmp t1 (rebalance_avl_wds t1))
+  (requires is_avl cmp (rebalance_avl_wdm t1))
+  (ensures equal cmp t1 (rebalance_avl_wdm t1))
   = admit ()
 
 (*
@@ -192,28 +193,34 @@ let rebalance_equal (#a: Type) (cmp: cmp a) (t1: bst a cmp)
   that is whether the size has increased
   => bad idea/bad design?
 *)
-
+//TODO: possibly a stronger invariant, not b ==> same "skeleton"
 #push-options "--z3rlimit 100"
 let rec insert_avl2_aux (#a: Type)
   (r:bool) (cmp:cmp a) (t: avl a cmp) (new_data: a)
-  : result:(avl a cmp & bool){
-    let t',b = result in
+  : Pure (avl a cmp & bool)
+  True
+  (fun (t', b) ->
     size_of_tree t' = size_of_tree t + (int_of_bool b) /\
-    height t <= height t' /\
-    height t' <= height t + 1 /\
+    hot_wdh t <= hot_wdh t' /\
+    hot_wdh t' <= hot_wdh t + 1 /\
     (b ==> add cmp t t' new_data) /\
-    (not b ==> equal cmp t t') /\
+    (not b ==>
+      //size_of_tree t == size_of_tree t' /\
+      height_of_tree t == height_of_tree t' /\
+      equal cmp t t'
+    ) /\
     (subset cmp t t')
-  }
+  )
   =
   match t with
-  | Leaf -> Node new_data Leaf Leaf 1, true
-  | Node data left right size ->
+  | Leaf ->
+      Node new_data Leaf Leaf 1 1, true
+  | Node data left right size height ->
     let delta = cmp new_data data in
     if delta = 0 then begin
       if r
       then
-        let new_t = Node new_data left right size in
+        let new_t = Node new_data left right size height in
         forall_keys_trans left
           (key_left cmp data)
           (key_left cmp new_data);
@@ -225,103 +232,126 @@ let rec insert_avl2_aux (#a: Type)
         t, false
     end
     else if delta < 0 then begin
-      //assert (subset cmp (fst (insert_avl2_aux r cmp left new_data))
-      //left);
       let new_left, b = insert_avl2_aux r cmp left new_data in
-      let new_size = size + (int_of_bool b) in
-      let new_t = Node data new_left right new_size in
-      // is_bst new_t
       if b then begin
+        let height_new_left = hot_wdh new_left in
+        let height_right = hot_wdh right in
+        let new_height = M.max height_new_left height_right + 1 in
+        let new_size = size + 1 in
+        assert (new_size = size + (int_of_bool b));
+        let new_t = Node data new_left right new_size new_height in
+        assert (is_wdm new_t);
         assert (add cmp left new_left new_data);
         add_preserves_cond cmp left new_left new_data
-          (key_left cmp data)
+          (key_left cmp data);
+        assert (forall_keys new_left (key_left cmp data));
+        assert (is_bst cmp new_t);
+
+        assert (is_avl cmp new_left);
+        assert (is_avl cmp right);
+        assert (hot_wdh t <= hot_wdh new_t);
+        assert (hot_wdh new_t <= hot_wdh t + 1);
+        rebalance_avl_wds_proof cmp new_t data;
+        assert (is_avl cmp (rebalance_avl_wdm new_t));
+        rebalance_avl_wds_size new_t;
+        rebalance_equal cmp new_t;
+        let new_t2 = rebalance_avl_wdm new_t in
+        new_t2, b
       end else begin
-        assert (equal cmp new_left left);
-        equal_preserves_cond cmp left new_left
-          (key_left cmp data)
-      end;
-      assert (forall_keys new_left (key_left cmp data));
-      assert (is_bst cmp new_t);
-
-
-      assert (is_avl cmp new_left);
-      assert (is_avl cmp right);
-      assert (height t <= height new_t);
-      assert (height new_t <= height t + 1);
-      rebalance_avl_wds_proof cmp new_t data;
-      assert (is_avl cmp (rebalance_avl_wds new_t));
-      rebalance_avl_wds_size new_t;
-      let new_t2 = rebalance_avl_wds new_t in
-      rebalance_equal cmp new_t;
-      //assert (subset cmp t new_t2);
-      //assert (b ==> add cmp t new_t2 new_data);
-      //assert (not b ==> equal cmp t new_t2);
-      //assert (height t <= height new_t2);
-      //assert (height new_t2 <= height t + 1);
-      new_t2, b
+        assert (size_of_tree new_left = size_of_tree left);
+        assert (height_of_tree new_left = height_of_tree left);
+        assert (is_balanced new_left);
+        assert (is_balanced right);
+        let new_t = Node data new_left right size height in
+        assert (is_balanced new_t);
+        assert (subset cmp new_left left);
+        subset_preserves_cond cmp new_left left (key_left cmp data);
+        assert (is_bst cmp new_t);
+        new_t, b
+        //assert (subset cmp t new_t2);
+        //assert (b ==> add cmp t new_t2 new_data);
+        //assert (not b ==> equal cmp t new_t2);
+        //assert (height t <= height new_t2);
+        //assert (height new_t2 <= height t + 1);
+        //new_t2, b
+      end
     end else begin
       let new_right, b = insert_avl2_aux r cmp right new_data in
-      let new_size = size + (int_of_bool b) in
-      let new_t = Node data left new_right new_size in
-       // is_bst new_t
       if b then begin
+        let height_left = hot_wdh left in
+        let height_new_right = hot_wdh new_right in
+        let new_height = M.max height_left height_new_right + 1 in
+        let new_size = size + 1 in
+        assert (new_size = size + (int_of_bool b));
+        let new_t = Node data left new_right new_size new_height in
+        assert (is_wdm new_t);
         assert (add cmp right new_right new_data);
         add_preserves_cond cmp right new_right new_data
-          (key_right cmp data)
-      end else begin
-        assert (equal cmp new_right right);
-        equal_preserves_cond cmp right new_right
-          (key_right cmp data)
-      end;
-      assert (forall_keys new_right (key_right cmp data));
-      assert (is_bst cmp new_t);
+          (key_right cmp data);
+        assert (forall_keys new_right (key_right cmp data));
+        assert (is_bst cmp new_t);
 
-      assert (is_avl cmp new_right);
-      assert (is_avl cmp left);
-      assert (height t <= height new_t);
-      assert (height new_t <= height t + 1);
-      rebalance_avl_wds_proof cmp new_t data;
-      assert (is_avl cmp (rebalance_avl_wds new_t));
-      rebalance_avl_wds_size new_t;
-      let new_t2 = rebalance_avl_wds new_t in
-      rebalance_equal cmp new_t;
-      //assert (subset cmp t new_t2);
-      //assert (b ==> add cmp t new_t2 new_data);
-      //assert (not b ==> equal cmp t new_t2);
-      //assert (height t <= height new_t2);
-      //assert (height new_t2 <= height t + 1);
-      new_t2, b
+        assert (is_avl cmp new_right);
+        assert (is_avl cmp left);
+        assert (hot_wdh t <= hot_wdh new_t);
+        assert (hot_wdh new_t <= hot_wdh t + 1);
+        rebalance_avl_wds_proof cmp new_t data;
+        assert (is_avl cmp (rebalance_avl_wdm new_t));
+        rebalance_avl_wds_size new_t;
+        rebalance_equal cmp new_t;
+        let new_t2 = rebalance_avl_wdm new_t in
+        new_t2, b
+      end else begin
+        assert (size_of_tree new_right = size_of_tree right);
+        assert (height_of_tree new_right = height_of_tree right);
+        assert (is_balanced left);
+        assert (is_balanced new_right);
+        let new_t = Node data left new_right size height in
+        assert (is_balanced new_t);
+        assert (subset cmp new_right right);
+        subset_preserves_cond cmp new_right right (key_right cmp data);
+        assert (is_bst cmp new_t);
+        new_t, b
+        //assert (subset cmp t new_t2);
+        //assert (b ==> add cmp t new_t2 new_data);
+        //assert (not b ==> equal cmp t new_t2);
+        //assert (height t <= height new_t2);
+        //assert (height new_t2 <= height t + 1);
+        //new_t2, b
+      end
     end
 #pop-options
 
-#push-options "--z3rlimit 50"
+#push-options "--z3rlimit 25"
 let rec remove_leftmost_avl (#a: Type0)
   (cmp:cmp a)
   (t: avl a cmp{Node? t})
-  : r:(avl a cmp & a){
+  : Pure (avl a cmp & a)
+  True
+  (fun (t', leftmost) ->
     //1 returned element was part of the tree
-    mem cmp t (snd r) = true /\
+    mem cmp t leftmost = true /\
     //2 returned element smaller than all elements of the new tree
-    forall_keys (fst r) (key_right cmp (snd r)) /\
+    forall_keys t' (key_right cmp leftmost) /\
     //3 returned element has been removed
-    mem cmp (fst r) (snd r) = false /\
+    mem cmp t' leftmost = false /\
     //4 rest of the tree preserved
+    add cmp t' t leftmost /\
+    //6 size decreased by 1
+    size_of_tree t' = size_of_tree t - 1 /\
+    //7
+    height_of_tree t - 1 <= height_of_tree t' /\
+    height_of_tree t' <= height_of_tree t
+  )
     //(forall x. cmp x (snd r) <> 0
     //  ==> mem cmp t x = mem cmp (fst r) x) /\
     //5 subset
     //subset cmp (fst r) t /\
-    add cmp (fst r) t (snd r) /\
-    //6 size decreased by 1
-    size_of_tree (fst r) = size_of_tree t - 1 /\
-    //7
-    height t - 1 <= height (fst r) /\
-    height (fst r) <= height t
     //Node? (fst r) ==> is_balanced (cleft (fst r)) /\
     //Node? (fst r) ==> is_balanced (cright (fst r)) /\
- }
   =
   match t with
-  | Node data Leaf right size ->
+  | Node data Leaf right size _ ->
       // (1 : trivial)
       // (2)
       assert (forall_keys right (key_right cmp data));
@@ -333,13 +363,16 @@ let rec remove_leftmost_avl (#a: Type0)
       //assert (height right <= 1);
       // (4 5 6 : trivial)
       right, data
-  | Node data left right size ->
+  | Node data left right size _ ->
       let new_left, leftmost = remove_leftmost_avl cmp left in
       // (1 : IH)
       assert (mem cmp left leftmost = true);
       assert (mem cmp t leftmost = true);
       // (2 : IH)
-      let new_t = Node data new_left right (size - 1) in
+      let height_new_left = hot_wdh new_left in
+      let height_right = hot_wdh right in
+      let new_height = M.max height_new_left height_right + 1 in
+      let new_t = Node data new_left right (size - 1) new_height in
       // new_left <= data
       add_is_subset cmp new_left left leftmost;
       assert (subset cmp new_left left);
@@ -354,13 +387,13 @@ let rec remove_leftmost_avl (#a: Type0)
         (key_right cmp leftmost);
       // (3 : use 2)
       //smaller_not_mem cmp new_t leftmost;
-      let new_t2 = rebalance_avl_wds new_t in
+      let new_t2 = rebalance_avl_wdm new_t in
       assert (is_balanced new_left);
       assert (is_balanced right);
-      assert (height left - 1 <= height new_left);
-      assert (height new_left <= height left);
-      assert (height right - height new_left <= 2);
-      assert (height new_left - height right <= 1);
+      assert (height_of_tree left - 1 <= height_of_tree new_left);
+      assert (height_of_tree new_left <= height_of_tree left);
+      assert (height_of_tree right - height_of_tree new_left <= 2);
+      assert (height_of_tree new_left - height_of_tree right <= 1);
       rebalance_avl_wds_proof cmp new_t data;
 
       // 1
@@ -379,52 +412,53 @@ let rec remove_leftmost_avl (#a: Type0)
       rebalance_avl_wds_size new_t;
       assert (size_of_tree new_t2 = size_of_tree t - 1);
       // 7
-      assert (height new_t2 <= height t);
-      assert (height t - 1 <= height new_t2);
+      assert (height_of_tree new_t2 <= height_of_tree t);
+      assert (height_of_tree t - 1 <= height_of_tree new_t2);
       assert (is_avl cmp new_t2);
       new_t2, leftmost
 #pop-options
 
 // https://en.wikipedia.org/wiki/Binary_search_tree#Deletion
-#push-options "--z3rlimit 80"
+#push-options "--z3rlimit 25"
 let delete_avl_aux0 (#a: Type0)
   (cmp:cmp a)
   (t: avl a cmp{Node? t})
   (data_to_rm: a{cmp (cdata t) data_to_rm = 0})
-  : r:bst a cmp
-  {
+  : Pure (bst a cmp)
+  True
+  (fun t' ->
     // 1 a b removal of one element
     mem cmp t data_to_rm = true /\
     //?data_to_rm = true /\
-    mem cmp r data_to_rm = false /\
+    mem cmp t' data_to_rm = false /\
     // 2 remaining tree unchanged
     //(forall x. cmp x data_to_rm <> 0
     //  ==> mem cmp t x = mem cmp r x) /\
-    add cmp r t data_to_rm /\
+    add cmp t' t data_to_rm /\
     // 3 size decreased by one
-    size_of_tree r = size_of_tree t - 1 /\
+    size_of_tree t' = size_of_tree t - 1 /\
     // 4
-    height t - 1 <= height r /\
-    height r <= height t
-  }
+    height_of_tree t - 1 <= height_of_tree t' /\
+    height_of_tree t' <= height_of_tree t
+  )
   =
   match t with
-  | Node data Leaf Leaf 1 -> Leaf
-  | Node data left Leaf size ->
+  | Node data Leaf Leaf 1 _ -> Leaf
+  | Node data left Leaf size _ ->
       assert (forall_keys left (key_left cmp data));
       equiv cmp left (key_left cmp data);
       //greater_not_mem cmp left data;
       assert (mem cmp left data = false);
       left
-  | Node data Leaf right size ->
+  | Node data Leaf right size _ ->
       assert (forall_keys right (key_right cmp data));
       equiv cmp right (key_right cmp data);
       //smaller_not_mem cmp right data;
       assert (mem cmp right data = false);
       right
   // successor of z = y
-  | Node z l (Node y Leaf x sy) sz ->
-      let r = Node y Leaf x sy in
+  | Node z l (Node y Leaf x sy hr) sz hz ->
+      let r = Node y Leaf x sy hr in
       // y <= x
       assert (forall_keys x (key_right cmp y));
       // l <= z <= y
@@ -432,7 +466,8 @@ let delete_avl_aux0 (#a: Type0)
         (key_left cmp z)
         (key_left cmp y);
       assert (forall_keys l (key_left cmp y));
-      let new_t = Node y l x (sz - 1) in
+      let new_height = M.max (hot_wdh l) (hr - 1) + 1 in
+      let new_t = Node y l x (sz - 1) new_height in
       // 3 is included
       assert (is_bst cmp new_t);
       //assert (size_of_tree new_t = size_of_tree t - 1);
@@ -464,13 +499,16 @@ let delete_avl_aux0 (#a: Type0)
       new_t
 
   // successor of z = to be retrieved
-  | Node z l r sz ->
+  | Node z l r sz hz ->
       assert (Node? r);
       // 1a
       assert (mem cmp t data_to_rm = true);
       // call to aux function, building new tree
       let new_right, succ_z = remove_leftmost_avl cmp r in
-      let new_t = Node succ_z l new_right (sz - 1) in
+      let height_new_right = hot_wdh new_right in
+      let height_left = hot_wdh l in
+      let new_height = M.max height_left height_new_right + 1 in
+      let new_t = Node succ_z l new_right (sz - 1) new_height in
       // left: l <= z <= succ_z
       // z <= succ_z
       assert (forall_keys r (key_right cmp z));
@@ -512,23 +550,25 @@ let delete_avl_aux0 (#a: Type0)
       new_t
 #pop-options
 
-let delete_avl_aux0_wo_refinement (#a: Type0)
-  (cmp:cmp a)
-  (t: avl a cmp{Node? t})
-  (data_to_rm: a{cmp (cdata t) data_to_rm = 0})
-  : r:bst a cmp
-  {
-    size_of_tree r = size_of_tree t - 1
-  }
-  = delete_avl_aux0 cmp t data_to_rm
+//let delete_avl_aux0_wo_refinement (#a: Type0)
+//  (cmp:cmp a)
+//  (t: avl a cmp{Node? t})
+//  (data_to_rm: a{cmp (cdata t) data_to_rm = 0})
+//  : r:bst a cmp
+//  {
+//    size_of_tree r = size_of_tree t - 1
+//  }
+//  = delete_avl_aux0 cmp t data_to_rm
 
-#push-options "--fuel 1 --ifuel 1 --z3rlimit 50"
+#push-options "--fuel 1 --ifuel 1 --z3rlimit 25"
 let delete_avl_aux1 (#a: Type0)
   (cmp:cmp a)
   (t: avl a cmp{Node? t})
   (data_to_rm: a{cmp (cdata t) data_to_rm = 0})
   //(t: avl a cmp{Node? t /\ cmp (cdata t) data_to_rm = 0})
-  : r:avl a cmp{
+  : Pure (avl a cmp)
+  True
+  (fun r ->
     // 1 a b removal of one element
     mem cmp t data_to_rm = true /\
     //?data_to_rm = true /\
@@ -540,37 +580,41 @@ let delete_avl_aux1 (#a: Type0)
     // 3 size decreased by one
     size_of_tree r = size_of_tree t - 1 /\
     // 4
-    height t - 1 <= height r /\
-    height r <= height t
-  }
+    height_of_tree t - 1 <= height_of_tree r /\
+    height_of_tree r <= height_of_tree t
+  )
   =
   let new_t1 = delete_avl_aux0 #a cmp t data_to_rm in
   match t with
-  | Node data Leaf Leaf 1 ->
+  | Node data Leaf Leaf 1 _ ->
       let new_t0 = Leaf
       in assert (new_t0 == new_t1);
       new_t0
-  | Node data left Leaf size ->
+  | Node data left Leaf size _ ->
       let new_t0 = left
       in assert (new_t0 == new_t1);
       new_t0
-  | Node data Leaf right size ->
+  | Node data Leaf right size _ ->
       let new_t0 = right
       in assert (new_t0 == new_t1);
       new_t0
   | _ ->
   let new_t0 = begin match t with
-  | Node z l (Node y Leaf x sy) sz ->
-      let new_t0 = Node y l x (sz - 1) in
+  | Node z l (Node y Leaf x _ hr) sz _ ->
+      let new_height = M.max (hot_wdh l) (hr - 1) + 1 in
+      let new_t0 = Node y l x (sz - 1) new_height in
       assert (is_balanced t);
       assert (is_balanced (cright t));
       assert (is_balanced (cright (cright t)));
       assert (is_balanced (cleft new_t0));
       assert (is_balanced (cright new_t0));
       new_t0
-  | Node z l r sz ->
+  | Node z l r sz _ ->
       let new_right, succ_z = remove_leftmost_avl cmp r in
-      let new_t0 = Node succ_z l new_right (sz - 1) in
+      let height_left = hot_wdh l in
+      let height_new_right = hot_wdh new_right in
+      let new_height = M.max height_left height_new_right + 1 in
+      let new_t0 = Node succ_z l new_right (sz - 1) new_height in
       assert (is_balanced (cleft new_t0));
       assert (is_balanced (cright new_t0));
       new_t0
@@ -579,9 +623,11 @@ let delete_avl_aux1 (#a: Type0)
   assert (new_t0 == new_t1);
   assert (is_balanced (cleft new_t0));
   assert (is_balanced (cright new_t0));
-  assert (height (cleft new_t0) - height (cright new_t0) <= 2);
-  assert (height (cright new_t0) - height (cleft new_t0) <= 2);
-  let new_t2 = rebalance_avl_wds new_t0 in
+  assert (height_of_tree (cleft new_t0)
+  - height_of_tree (cright new_t0) <= 2);
+  assert (height_of_tree (cright new_t0)
+  - height_of_tree (cleft new_t0) <= 2);
+  let new_t2 = rebalance_avl_wdm new_t0 in
   assert (is_bst cmp new_t0);
   rebalance_avl_wds_proof cmp new_t0 (cdata new_t0);
   assert (is_avl cmp new_t2);
@@ -597,46 +643,91 @@ let delete_avl_aux1 (#a: Type0)
   rebalance_avl_wds_size new_t0;
   assert (size_of_tree new_t2 = size_of_tree new_t0);
   // 4
-  assert (height t - 1 <= height new_t0);
-  assert (height new_t0 <= height t);
-  assert (height t - 1 <= height new_t2);
-  assert (height new_t2 <= height t);
+  assert (height_of_tree t - 1 <= height_of_tree new_t0);
+  assert (height_of_tree new_t0 <= height_of_tree t);
+  assert (height_of_tree t - 1 <= height_of_tree new_t2);
+  assert (height_of_tree new_t2 <= height_of_tree t);
 
   new_t2
 #pop-options
 
-#push-options "--z3rlimit 50"
+//let rec delete_avl_aux (#a: Type0)
+//  (cmp:cmp a) (t: avl a cmp) (data_to_rm: a)
+//  : wdm a & bool
+//  =
+//  match t with
+//  | Leaf -> Leaf, false
+//  | Node data left right size height ->
+//      let delta = cmp data_to_rm data in
+//      if delta < 0 then begin
+//        let new_left, b = delete_avl_aux cmp left data_to_rm in
+//        let new_size = size - (int_of_bool b) in
+//        let height_new_left = height_of_tree new_left in
+//        let height_right = height_of_tree right in
+//        let new_height = M.max height_new_left height_right + 1 in
+//        let new_t = Node data new_left right new_size new_height in
+//        let new_t2 = rebalance_avl_wdm new_t in
+//        new_t2, b
+//      end else if delta > 0 then begin
+//        let new_right, b = delete_avl_aux cmp right data_to_rm in
+//        let new_size = size - (int_of_bool b) in
+//        let height_left = hot_wdh left in
+//        let height_new_right = hot_wdh new_right in
+//        let new_height = M.max height_left height_new_right + 1 in
+//        let new_t = Node data left new_right new_size new_height in
+//        let new_t2 = rebalance_avl_wdm new_t in
+//        new_t2, b
+//     end else begin
+//        let new_t = delete_avl_aux1 cmp t data_to_rm in
+//        new_t, true
+//     end
+
+#push-options "--z3rlimit 200"
 let rec delete_avl_aux (#a: Type0)
   (cmp:cmp a) (t: avl a cmp) (data_to_rm: a)
-  : result:(avl a cmp & bool){
-    let t',b = result in
+  : Pure (avl a cmp & bool)
+  True
+  (fun (t',b) ->
     size_of_tree t' = size_of_tree t - (int_of_bool b) /\
     subset cmp t' t /\
-    height t - 1 <= height t' /\
-    height t' <= height t /\
+    height_of_tree t - 1 <= height_of_tree t' /\
+    height_of_tree t' <= height_of_tree t /\
     (b ==> add cmp t' t data_to_rm) /\
     ((not b) ==> equal cmp t' t) /\
     mem cmp t' data_to_rm = false
-  }
+  )
   =
   match t with
   | Leaf -> Leaf, false
-  | Node data left right size ->
+  | Node data left right size height ->
       let delta = cmp data_to_rm data in
       if delta < 0 then begin
         let new_left, b = delete_avl_aux cmp left data_to_rm in
-        assert (is_avl cmp new_left);
+
+        let new_size = size - (int_of_bool b) in
+        let height_new_left = hot_wdh new_left in
+        let height_right = hot_wdh right in
+        let new_height = M.max height_new_left height_right + 1 in
+        let new_t = Node data new_left right new_size new_height in
+        assert (is_wdm new_t);
+
         assert (forall_keys left (key_left cmp data));
         assert (subset cmp new_left left);
         subset_preserves_cond cmp new_left left (key_left cmp data);
         assert (forall_keys new_left (key_left cmp data));
-        let new_size = size - (int_of_bool b) in
-        let new_t = Node data new_left right new_size in
+        assert (forall_keys right (key_right cmp data));
+        assert (is_bst cmp new_t);
 
-        rebalance_avl_wds_size new_t;
+        assert (is_balanced new_left);
+        assert (is_balanced right);
+        assert (height_of_tree new_left - height_of_tree right <= 2);
+        assert (height_of_tree right - height_of_tree new_left <= 2);
+        let new_t2 = rebalance_avl_wdm new_t in
         rebalance_avl_wds_proof cmp new_t data;
-        let new_t2 = rebalance_avl_wds new_t in
-        rebalance_equal cmp new_t;
+        assert (is_avl cmp new_t2);
+        //admit ();
+        //assume (height_of_tree t - 1 <= height_of_tree new_t2);
+        //assume (height_of_tree new_t2 <= height_of_tree t);
 
         assert (mem cmp new_left data_to_rm = false);
         forall_keys_trans right
@@ -644,23 +735,38 @@ let rec delete_avl_aux (#a: Type0)
           (key_right cmp data_to_rm);
         smaller_not_mem cmp right data_to_rm;
         assert (mem cmp new_t data_to_rm = false);
+        rebalance_equal cmp new_t;
         assert (mem cmp new_t2 data_to_rm = false);
+        rebalance_avl_wds_size new_t;
 
         new_t2, b
-      end
-      else if delta > 0 then begin
+
+      end else if delta > 0 then begin
         let new_right, b = delete_avl_aux cmp right data_to_rm in
-        assert (is_avl cmp new_right);
+
+        let new_size = size - (int_of_bool b) in
+        let height_left = hot_wdh left in
+        let height_new_right = hot_wdh new_right in
+        let new_height = M.max height_left height_new_right + 1 in
+        let new_t = Node data left new_right new_size new_height in
+        assert (is_wdm new_t);
+
         assert (forall_keys right (key_right cmp data));
         assert (subset cmp new_right right);
         subset_preserves_cond cmp new_right right (key_right cmp data);
         assert (forall_keys new_right (key_right cmp data));
-        let new_size = size - (int_of_bool b) in
-        let new_t = Node data left new_right new_size in
-        rebalance_avl_wds_size new_t;
+        assert (is_bst cmp new_t);
+
+        assert (is_balanced left);
+        assert (is_balanced new_right);
+        assert (height_of_tree left - height_of_tree new_right <= 2);
+        assert (height_of_tree new_right - height_of_tree left <= 2);
+        let new_t2 = rebalance_avl_wdm new_t in
         rebalance_avl_wds_proof cmp new_t data;
-        let new_t2 = rebalance_avl_wds new_t in
-        rebalance_equal cmp new_t;
+        assert (is_avl cmp new_t2);
+        //admit ();
+        //assume (height_of_tree t - 1 <= height_of_tree new_t2);
+        //assume (height_of_tree new_t2 <= height_of_tree t);
 
         assert (mem cmp new_right data_to_rm = false);
         forall_keys_trans left
@@ -668,23 +774,27 @@ let rec delete_avl_aux (#a: Type0)
           (key_left cmp data_to_rm);
         greater_not_mem cmp left data_to_rm;
         assert (mem cmp new_t data_to_rm = false);
+        rebalance_equal cmp new_t;
         assert (mem cmp new_t2 data_to_rm = false);
+        rebalance_avl_wds_size new_t;
 
         new_t2, b
-      end
-      else
+      end else begin
         let new_t = delete_avl_aux1 cmp t data_to_rm in
         new_t, true
+      end
 #pop-options
 
 let insert_avl2 (#a: Type)
   (r:bool) (cmp:cmp a) (t: avl a cmp) (new_data: a)
-  : avl a cmp
-//  {
-//    let _,b = insert_avl2_aux r cmp t new_data in
-//    size_of_tree t' = size_of_tree t + (int_of_bool b) /\
-//    add cmp t t' new_data
-//  }
+  : Pure (avl a cmp)
+  True
+  (fun t' ->
+    let _,b = insert_avl2_aux r cmp t new_data in
+    size_of_tree t' = size_of_tree t + (int_of_bool b) /\
+    b ==> add cmp t t' new_data /\
+    (not b) ==> equal cmp t t'
+  )
   = fst (insert_avl2_aux r cmp t new_data)
 
 let delete_avl (#a: Type0)
@@ -699,7 +809,7 @@ let rec lemma_insert (#a: Type)
   (ensures snd (insert_avl2_aux r cmp t new_data) = true)
   = match t with
   | Leaf -> ()
-  | Node data left right _ ->
+  | Node data left right _ _ ->
       let delta = cmp new_data data in
       if delta = 0 then begin
         test_aux0 cmp t data new_data;
@@ -716,7 +826,7 @@ let rec lemma_delete (#a: Type)
   (ensures snd (delete_avl_aux cmp t data_to_rm) = true)
   = match t with
   | Leaf -> ()
-  | Node data left right _ ->
+  | Node data left right _ _ ->
       let delta = cmp data_to_rm data in
       if delta < 0 then begin
         unicity_left cmp t data_to_rm;
