Spec.Trees.fst
@@ -1,29 +1,28 @@
 module Spec.Trees
 
+module M = FStar.Math.Lib
+
 (*** Type definitions *)
 
 (**** The tree structure *)
 
 type tree (a: Type) =
   | Leaf : tree a
-  | Node: data: a -> left: tree a -> right: tree a -> size: nat -> tree a
+  | Node:
+    data: a ->
+    left: tree a -> right: tree a ->
+    size: nat -> height: nat -> tree a
 
 let cdata (#a: Type) (t: tree a{Node? t}) =
-  let Node d _ _ _ = t in d
+  let Node d _ _ _ _ = t in d
 let cleft (#a: Type) (t: tree a{Node? t}) =
-  let Node _ l _ _ = t in l
+  let Node _ l _ _ _ = t in l
 let cright (#a: Type) (t: tree a{Node? t}) =
-  let Node _ _ r _ = t in r
+  let Node _ _ r _ _ = t in r
 let csize (#a: Type) (t: tree a{Node? t}) =
-  let Node _ _ _ s = t in s
-
-(**** Binary search trees *)
-
-//@Trees
-let rec size_of_tree (#a: Type) (x: tree a) : Tot nat (decreases x) =
-  match x with
-  | Leaf -> 0
-  | Node _ left right _ -> size_of_tree left + size_of_tree right + 1
+  let Node _ _ _ s _ = t in s
+let cheight (#a: Type) (t: tree a{Node? t}) =
+  let Node _ _ _ _ h = t in h
 
 //@Trees.Misc
 let proj (x: int) : r:int{-1 <= r /\ r <= 1}
@@ -31,18 +30,28 @@ let proj (x: int) : r:int{-1 <= r /\ r <= 1}
     else if x = 0 then 0
     else 1
 
+(**** Binary search trees *)
+
+//@Trees
+let rec size_of_tree (#a: Type) (x: tree a) : nat
+  = match x with
+  | Leaf -> 0
+  | Node _ left right _ _ ->
+      size_of_tree left + size_of_tree right + 1
+
 //@Trees
 (* is with defined size *)
 let rec is_wds (#a: Type) (x: tree a)
-  : GTot bool (decreases x) =
-  match x with
+  : GTot bool
+  = match x with
   | Leaf -> true
-  | Node data left right size ->
+  | Node data left right size _ ->
       let s1 = size_of_tree left in
       let s2 = size_of_tree right in
       let b1 = is_wds left in
       let b2 = is_wds right in
       let s = s1 + s2 + 1 in
+      assert (s = size_of_tree x);
       b1 && b2 && size = s
 
 //@Trees
@@ -51,23 +60,60 @@ let wds (a: Type) = x:tree a {is_wds x}
 (**** Height *)
 
 //@Trees
-let rec height (#a: Type) (x: tree a) : nat =
+let rec height_of_tree_old (#a: Type) (x: tree a) : nat =
   match x with
   | Leaf -> 0
-  | Node data left right _ ->
-    let hleft = height left in
-    let hright = height right in
-    if hleft > hright then hleft + 1
-    else hright + 1
+  | Node _ left right _ _ ->
+      let hleft = height_of_tree_old left in
+      let hright = height_of_tree_old right in
+      if hleft > hright then hleft + 1
+      else hright + 1
+
+let rec height_of_tree (#a: Type) (x:tree a) : nat =
+  match x with
+  | Leaf -> 0
+  | Node _ left right _ _ ->
+      (M.max (height_of_tree left) (height_of_tree right)) + 1
+
+let rec height_equal (#a: Type) (x:tree a)
+  : Lemma
+  (height_of_tree_old x = height_of_tree x)
+  = match x with
+  | Leaf -> ()
+  | Node _ left right _ _ ->
+      let hleft = height_of_tree left in
+      height_equal left;
+      assert (hleft = height_of_tree_old left);
+      let hright = height_of_tree right in
+      height_equal right;
+      assert (hright = height_of_tree_old right);
+      let m = M.max (hleft + 1) (hright + 1) in
+      assert (m = height_of_tree_old x)
+
+(* is with defined height *)
+let rec is_wdh (#a: Type) (x: tree a)
+  : GTot bool
+  = match x with
+  | Leaf -> true
+  | Node data left right _ height ->
+      let h1 = height_of_tree left in
+      let h2 = height_of_tree right in
+      let b1 = is_wdh left in
+      let b2 = is_wdh right in
+      let h = (M.max h1 h2) + 1 in
+      assert (h = height_of_tree x);
+      b1 && b2 && height = h
+
+let wdh (a: Type) = x:tree a {is_wdh x}
 
 //@Trees.Misc
 let rec height_lte_size (#a: Type) (t: tree a)
   : Lemma
-  (height t <= size_of_tree t)
+  (height_of_tree t <= size_of_tree t)
   =
   match t with
   | Leaf -> ()
-  | Node data left right _ ->
+  | Node data left right _ _ ->
       height_lte_size left;
       height_lte_size right
 
@@ -82,10 +128,21 @@ let get (#a: Type) (v: option a{Some? v}) : a =
 
 //@Trees
 let sot_wds (#a: Type) (t: wds a)
-  : s:nat{size_of_tree t == s} =
+  : s:nat{size_of_tree t = s} =
   match t with
   | Leaf -> 0
-  | Node _ _ _ s -> s
+  | Node _ _ _ s _ -> s
+
+let hot_wdh (#a: Type) (t: wdh a)
+  : h:nat{height_of_tree t = h} =
+  match t with
+  | Leaf -> 0
+  | Node _ _ _ _ h -> h
+
+(* is with defined metadata *)
+let is_wdm (#a: Type) (t: tree a) : GTot bool
+  = is_wds t && is_wdh t
+let wdm (a: Type) = x:tree a {is_wdm x}
 
 
 (*
@@ -99,16 +156,20 @@ t1   z   =>   x   t3
 //  match r with
 //  | Node x t1 (Node z t2 t3 _) _ -> Some (Node z (Node x t1 t2 0) t3 0)
 //  | _ -> None
-let rotate_left_wds (#a: Type) (r: wds a) : option (wds a) =
+let rotate_left_wdm (#a: Type) (r: wdm a) : option (wdm a) =
   match r with
-  | Node x t1 (Node z t2 t3 _) s ->
+  | Node x t1 (Node z t2 t3 _ _) s _ ->
       let s12 = sot_wds t1 + sot_wds t2 + 1 in
-      let t12 = Node x t1 t2 s12 in
-      //induction_wds x t1 t2;
-      assert (is_wds t12);
+      let h1 = hot_wdh t1 in
+      let h2 = hot_wdh t2 in
+      let h3 = hot_wdh t3 in
+      let h12 = (M.max h1 h2) + 1 in
+      let t12 = Node x t1 t2 s12 h12 in
+      assert (is_wdm t12);
       let s123 = s12 + sot_wds t3 + 1 in
       assert (s123 == s);
-      Some (Node z t12 t3 s)
+      let h123 = (M.max h12 h3) + 1 in
+      Some (Node z t12 t3 s h123)
   | _ -> None
 
 (*
@@ -123,16 +184,20 @@ t1 t2          t2 t3
 //  | Node x (Node z t1 t2 _) t3 _ ->
 //      Some (Node z t1 (Node x t2 t3 0) 0)
 //  | _ -> None
-let rotate_right_wds (#a: Type) (r: wds a) : option (wds a) =
+let rotate_right_wdm (#a: Type) (r: wdm a) : option (wdm a) =
   match r with
-  | Node x (Node z t1 t2 _) t3 s ->
+  | Node x (Node z t1 t2 _ _) t3 s _ ->
       let s23 = sot_wds t2 + sot_wds t3 + 1 in
-      let t23 = Node x t2 t3 s23 in
-      //induction_wds x t2 t3;
-      assert (is_wds t23);
+      let h1 = hot_wdh t1 in
+      let h2 = hot_wdh t2 in
+      let h3 = hot_wdh t3 in
+      let h23 = (M.max h2 h3) + 1 in
+      let t23 = Node x t2 t3 s23 h23 in
+      assert (is_wdm t23);
       let s123 = sot_wds t1 + s23 + 1 in
       assert (s123 == s);
-      Some (Node z t1 t23 s)
+      let h123 = (M.max h1 h23) + 1 in
+      Some (Node z t1 t23 s h123)
   | _ -> None
 
 (*
@@ -148,20 +213,25 @@ t1     z    =>   x     z
 //  | Node x t1 (Node z (Node y t2 t3 _) t4 _) _ ->
 //      Some (Node y (Node x t1 t2 0) (Node z t3 t4 0) 0)
 //  | _ -> None
-let rotate_right_left_wds (#a: Type) (r: wds a) : option (wds a) =
+let rotate_right_left_wdm (#a: Type) (r: wdm a) : option (wdm a) =
   match r with
-  | Node x t1 (Node z (Node y t2 t3 _) t4 _) s ->
+  | Node x t1 (Node z (Node y t2 t3 _ _) t4 _ _) s _ ->
       let s12 = sot_wds t1 + sot_wds t2 + 1 in
-      let t12 = Node x t1 t2 s12 in
-      //induction_wds x t1 t2;
-      assert (is_wds t12);
+      let h1 = hot_wdh t1 in
+      let h2 = hot_wdh t2 in
+      let h12 = M.max h1 h2 + 1 in
+      let t12 = Node x t1 t2 s12 h12 in
+      assert (is_wdm t12);
       let s34 = sot_wds t3 + sot_wds t4 + 1 in
-      let t34 = Node z t3 t4 s34 in
-      //induction_wds z t3 t4;
-      assert (is_wds t34);
+      let h3 = hot_wdh t3 in
+      let h4 = hot_wdh t4 in
+      let h34 = M.max h3 h4 + 1 in
+      let t34 = Node z t3 t4 s34 h34 in
+      assert (is_wdm t34);
       let s1234 = s12 + s34 + 1 in
+      let h1234 = M.max h12 h34 + 1 in
       assert (s1234 == s);
-      Some (Node y t12 t34 s)
+      Some (Node y t12 t34 s h1234)
   | _ -> None
 
 (*
@@ -176,43 +246,48 @@ t1   y         t1 t2 t3 t4
 //  match r with
 //  | Node x (Node z t1 (Node y t2 t3 _) _) t4 _  -> Some (Node y (Node z t1 t2 0) (Node x t3 t4 0) 0)
 //  | _ -> None
-let rotate_left_right_wds (#a: Type) (r: wds a) : option (wds a) =
+let rotate_left_right_wdm (#a: Type) (r: wdm a) : option (wdm a) =
   match r with
-  | Node x (Node z t1 (Node y t2 t3 _) _) t4 s ->
+  | Node x (Node z t1 (Node y t2 t3 _ _) _ _) t4 s _ ->
       let s12 = sot_wds t1 + sot_wds t2 + 1 in
-      let t12 = Node z t1 t2 s12 in
-      //induction_wds z t1 t2;
-      assert (is_wds t12);
+      let h1 = hot_wdh t1 in
+      let h2 = hot_wdh t2 in
+      let h12 = M.max h1 h2 + 1 in
+      let t12 = Node z t1 t2 s12 h12 in
+      assert (is_wdm t12);
       let s34 = sot_wds t3 + sot_wds t4 + 1 in
-      let t34 = Node x t3 t4 s34 in
-      //induction_wds x t3 t4;
-      assert (is_wds t34);
+      let h3 = hot_wdh t3 in
+      let h4 = hot_wdh t4 in
+      let h34 = M.max h3 h4 + 1 in
+      let t34 = Node x t3 t4 s34 h34 in
+      assert (is_wdm t34);
       let s1234 = s12 + s34 + 1 in
       assert (s1234 == s);
-      Some (Node y t12 t34 s)
+      let h1234 = M.max h12 h34 + 1 in
+      Some (Node y t12 t34 s h1234)
   | _ -> None
 
 //@Trees/AVL
-let rotate_left_size (#a: Type) (r: wds a)
+let rotate_left_size (#a: Type) (r: wdm a)
   : Lemma
-  (requires Some? (rotate_left_wds r))
-  (ensures size_of_tree (get (rotate_left_wds r)) == size_of_tree r)
+  (requires Some? (rotate_left_wdm r))
+  (ensures size_of_tree (get (rotate_left_wdm r)) == size_of_tree r)
   = ()
-let rotate_right_size (#a: Type) (r: wds a)
+let rotate_right_size (#a: Type) (r: wdm a)
   : Lemma
-  (requires Some? (rotate_right_wds r))
-  (ensures size_of_tree (get (rotate_right_wds r)) == size_of_tree r)
+  (requires Some? (rotate_right_wdm r))
+  (ensures size_of_tree (get (rotate_right_wdm r)) == size_of_tree r)
   = ()
-let rotate_right_left_size (#a: Type) (r: wds a)
+let rotate_right_left_size (#a: Type) (r: wdm a)
   : Lemma
-  (requires Some? (rotate_right_left_wds r))
+  (requires Some? (rotate_right_left_wdm r))
   (ensures
-  size_of_tree (get (rotate_right_left_wds r)) == size_of_tree r)
+  size_of_tree (get (rotate_right_left_wdm r)) == size_of_tree r)
   = ()
-let rotate_left_right_size (#a: Type) (r: wds a)
+let rotate_left_right_size (#a: Type) (r: wdm a)
   : Lemma
-  (requires Some? (rotate_left_right_wds r))
+  (requires Some? (rotate_left_right_wdm r))
   (ensures
-  size_of_tree (get (rotate_left_right_wds r)) == size_of_tree r)
+  size_of_tree (get (rotate_left_right_wdm r)) == size_of_tree r)
   = ()
 
